

IML - Ex-3

Omri Melcer

December 15, 2025

1. Let $f(x) = ax + b$ we will show that f is convex. Let $x, y \in \mathbb{R}, t \in [0, 1]$.

$$f(tx + (1-t)y) = atx + a(1-t)y + b = atx + a(1-t)y + tb + (1-t)b = t*(f(x)) + (1-t)f(y)$$

2. We will prove that $f(x) = ax^2 + bx + c$ is convex $\iff a \geq 0$:

- (a) $f(x)$ is convex $\implies a \geq 0$. we will take $x = 1, y = -1$ and $t = \frac{1}{2}$ then we know that

$$f(tx + (1-t)y) = f(0) = c \leq \frac{1}{2}f(-1) + \frac{1}{2}f(1) = \frac{a1^2 - bc + c + ac^2 + bc + c}{2} = a + c \implies 0 \leq a$$

- (b) $a \geq 0 \implies f(x)$ is convex Let $x, y \in \mathbb{R}$ and $t \in [0, 1]$. we will show that

$$\Delta = t(f(x) + (1-t)f(y) - [f(tx + (1-t)y)]) \geq 0$$

$$f(tx + (1-t)y) = a(tx + (1-t)y)^2 + b(tx + (1-t)y) + c$$

like in section 1 the $b(tx + (1-t)y) + c$ will be cancelled from both side in Δ . Thus we get

$$\Delta = [at^2x^2 - 2at(t-1)xy + a(1-t)^2y^2] - tax^2 - (1-t)ay^2$$

we pull out a and group by x^2, y^2, xy

$$\Delta = a \left[x^2(t^2 - t) + 2xy(t^2 - t) + y^2 \underbrace{[(1-t)^2 - (1-t)]}_{=1-2t+t^2-1+t=t^2-t} \right] = \underbrace{a}_{\geq 0} * \underbrace{t}_{\geq 0} * \underbrace{(1-t)}_{\geq 0} \underbrace{(x-y)^2}_{\geq 0} \geq 0$$

3. $f(x) = e^x$ is convex. The most standard way to prove this is by second derivative since $f''(x) = e^x \geq 0$. Since we only use the algebraic definition, Let $x, y \in \mathbb{R}, t \in [0, 1]$.

$$f(tx + (1-t)y) = e^{tx + (1-t)y} = e^{tx} * e^{(1-t)y}$$

both $e^x = u, e^y = v$ are non-negative then by the young inequality:

$$e^{tx} * e^{(1-t)y} = u^t v^{1-t} \leq tu * (1-t)v = tf(x) + (1-t)f(y)$$

4. Let $c \in \mathbb{R}$ $f(x) = \max(x, c) = \begin{cases} c & x \leq c \\ x & \text{else} \end{cases}$. Let $x, y \in \mathbb{R}, t \in [0, 1]$.

(a) case 1: $x \leq c, y \leq c \implies tx + (1-t)y \leq c \implies f(tx + (1-t)y) = c$
thus:

$$t(f(x)) + (1-t)f(y) = c \geq c$$

(b) case 2: $x, y \geq c$ this is a linear function which we already proved is convex.

(c) case 3: WLG $x \leq c$ and $y \geq c$ thus $f(x) = c$ $f(y) = y$.

$$tf(x) + (1-t)f(y) = tc + (1-t)y$$

but also

$$tc + (1-t)y \geq tc + (1-t)c = c$$

Thus

$$\max(c, tc + (1-t)y) \leq tf(x) + (1-t)f(y)$$

5. We will show a counter example to $f(x) = \cos(x)$ with $t = \frac{1}{2}$ and $x = -\frac{\pi}{2}$ and $y = \frac{\pi}{2}$ thus on the left side we get $\cos(0) = 1$ and on the right side we get

$$\frac{\cos(-\frac{\pi}{2}) + \cos(\frac{\pi}{2})}{2} = 0 \not\geq 1$$